\documentclass{article}
\usepackage{amsmath}
\begin{document}

\section{Normal Form}
\large{$$((\lambda a.(\lambda b.b\ b)\ (\lambda b.b\ b))\ b)\ ((\lambda c.(c\ b))\ (\lambda a.a))\rightarrow_\beta$$}
\large{$$((\lambda b.b\ b)\ (\lambda b.b\ b))\ ((\lambda c.(c\ b))\ (\lambda a.a))\rightarrow_\beta$$}
\large{$$((\lambda b.b\ b)\ (\lambda b.b\ b))\ ((\lambda c.(c\ b))\ (\lambda a.a))\rightarrow_\beta$$}
\large{$$((\lambda b.b\ b)\ (\lambda b.b\ b))\ ((\lambda a.a)\ b)\rightarrow_\beta$$}
\large{$$((\lambda b.b\ b)\ (\lambda b.b\ b))\ b\rightarrow_\beta$$}
\large{$$((\lambda b.b\ b)\ (\lambda b.b\ b))\ b\rightarrow_\beta$$}
$$\hdots$$

\section{S S K}
$$\textbf{I} \equiv \lambda x.x$$
$$K \equiv \lambda x\ y.x$$
$$S \equiv \lambda x\ y\ z. x\ z\ (y\ z)$$

\large{$$(\lambda x\ y\ z. x\ z\ (y\ z))\ (\lambda a\ b.a)\ (\lambda a\ b.a)\rightarrow_\beta$$}
\large{$$(\lambda y\ z. (\lambda a\ b.a)\ z\ (y\ z))\ (\lambda a\ b.a)\rightarrow_\beta$$}
\large{$$\lambda z. (\lambda a\ b.a)\ z\ ((\lambda a\ b.a)\ z)\rightarrow_\beta$$}
\large{$$\lambda z. (\lambda b.z)\ ((\lambda a\ b.a)\ z)\rightarrow_\beta$$}
\large{$$\lambda z. z$$}

\end{document}
